thys/Isabelle_Meta_Model/isabelle_home/src/HOL/Isabelle_Main2.thy
@@ -34,7 +34,6 @@
  * (INCLUDING NEGLIGENCE OR OTHERWISE) ARISING IN ANY WAY OUT OF THE USE
  * OF THIS SOFTWARE, EVEN IF ADVISED OF THE POSSIBILITY OF SUCH DAMAGE.
  ******************************************************************************)
-(* $Id:$ *)
 
 theory   Isabelle_Main2
 imports  "../Pure/Isar/Isabelle_typedecl"
