thys/Isabelle_Meta_Model/meta_isabelle/Meta_Pure.thy
@@ -34,7 +34,6 @@
  * (INCLUDING NEGLIGENCE OR OTHERWISE) ARISING IN ANY WAY OUT OF THE USE
  * OF THIS SOFTWARE, EVEN IF ADVISED OF THE POSSIBILITY OF SUCH DAMAGE.
  ******************************************************************************)
-(* $Id:$ *)
 
 section\<open>(Pure) Term Meta-Model aka. AST definition of (Pure) Term\<close>
 
