thys/Isabelle_Meta_Model/toy_example/Toy_Library_Static.thy
@@ -34,7 +34,6 @@
  * (INCLUDING NEGLIGENCE OR OTHERWISE) ARISING IN ANY WAY OUT OF THE USE
  * OF THIS SOFTWARE, EVEN IF ADVISED OF THE POSSIBILITY OF SUCH DAMAGE.
  ******************************************************************************)
-(* $Id:$ *)
 
 chapter\<open>Toy Libraries Static\<close>
 section\<open>Main Common Static Libraries\<close>
