thys/Isabelle_Meta_Model/toy_example/embedding/meta_toy/Meta_Toy_extended.thy
@@ -34,7 +34,6 @@
  * (INCLUDING NEGLIGENCE OR OTHERWISE) ARISING IN ANY WAY OUT OF THE USE
  * OF THIS SOFTWARE, EVEN IF ADVISED OF THE POSSIBILITY OF SUCH DAMAGE.
  ******************************************************************************)
-(* $Id:$ *)
 
 section\<open>Toy Meta-Model aka. AST definition of Toy (II)\<close>
 
