thys/Isabelle_Meta_Model/toy_example/embedding/meta_toy/Parser_META.thy
@@ -34,7 +34,6 @@
  * (INCLUDING NEGLIGENCE OR OTHERWISE) ARISING IN ANY WAY OUT OF THE USE
  * OF THIS SOFTWARE, EVEN IF ADVISED OF THE POSSIBILITY OF SUCH DAMAGE.
  ******************************************************************************)
-(* $Id:$ *)
 
 section\<open>Instantiating the Parser of META\<close>
 
@@ -313,17 +312,14 @@ definition of_bool where "of_bool b = case_bool
   (b \<open>false\<close>)"
 
 definition' \<open>sml_escape =
-  String.replace_chars ((* (* ERROR code_reflect *)
-                        \<lambda> Char Nibble0 NibbleA \<Rightarrow> \<open>\n\<close>
-                        | Char Nibble0 Nibble5 \<Rightarrow> \<open>\005\<close>
-                        | Char Nibble0 Nibble6 \<Rightarrow> \<open>\006\<close>
-                        | Char Nibble7 NibbleF \<Rightarrow> \<open>\127\<close>
-                        | x \<Rightarrow> \<degree>x\<degree>*)
-                        \<lambda>x. if x = Char Nibble0 NibbleA then \<open>\n\<close>
+  String.replace_chars (\<lambda>x. if x = Char Nibble0 NibbleA then \<open>\n\<close>
                             else if x = Char Nibble0 Nibble5 then \<open>\005\<close>
                             else if x = Char Nibble0 Nibble6 then \<open>\006\<close>
                             else if x = Char Nibble7 NibbleF then \<open>\127\<close>
                             else \<degree>x\<degree>)\<close>
+text \<open>Because of @{theory "Code_Char"}, it is not possible of extracting
+@{term "\<lambda> Char Nibble0 NibbleA \<Rightarrow> \<open>\<close>
+        | x \<Rightarrow> \<degree>x\<degree>"}.\<close>
 
 definition' \<open>of_string a b =
  (\<lambda>x. b (S.flatten [ \<open>(META.SS_base (META.ST "\<close>
